rocq-osiris/theories/program_logic/pure/binding_rules.v
@@ -10,12 +10,12 @@ From osiris.program_logic.pure Require Import wp pure_rules judgements pattern_r
 Definition bindings η bs (φ : env -> Prop) (ψ : exn -> Prop) :=
   pure (eval_bindings η bs) φ ψ.
 
-Lemma pure_irrefutably_extend {E} η δ p v φ (ψ : E → Prop) :
-  pure (eval_pat η δ p v) φ ⊥ →
+Lemma pure_irrefutably_extend `{Observe B E} η δ p v (φ : env → Prop) (ψ : B → Prop) :
+  pure (eval_pat η δ p v) φ (⊥ : unit → Prop) →
   pure (irrefutably_extend η δ p v) φ ψ.
 Proof.
-  intros H.
-  apply pure_wp_try, (pure_wp_mono _ H);
+  intros Hpat.
+  apply pure_wp_try, (pure_wp_mono _ Hpat);
     firstorder eauto with pure.
 Qed.
 
@@ -24,7 +24,7 @@ Qed.
 (* Syntax-directed reasoning rules for the auxiliary judgement [bindings]. *)
 
 Lemma bindings_cons_unary `{Encode A} η p e bs φ :
-  pure (eval η e) (λ a : A, bindings η bs (λ η', pattern η η' p #a φ False) ⊥) ⊥ ->
+  pure (eval η e) (λ a : A, bindings η bs (λ η', pattern η η' p #a φ False) ⊥) (⊥ : exn → Prop) ->
   bindings η (Binding p e :: bs) φ ⊥.
 Proof.
   unfold bindings. simpl. intros He.
@@ -33,6 +33,8 @@ Proof.
   eapply pure_ret_mono. { apply He. } intros a Ha.
   eapply pure_ret_mono. { apply Ha. } intros η' Hpat.
   apply pure_irrefutably_extend. apply Hpat.
+  Unshelve. all: eauto with pure.
+  exact _.
 Qed.
 
 Lemma bindings_cons `{Encode A} η p e bs (φ1 : A -> Prop) φ2 φ ψ :
@@ -71,19 +73,16 @@ Proof.
   eapply pure_ret; eauto.
 Qed.
 
-Lemma bindings_pair `{Encode A, Encode B} η p1 p2 e bs φ φ'
-  (φ1 : A -> Prop) (φ2 : B -> Prop) ψ :
-  pure (eval η e) (λ '(a, b), φ1 a /\ φ2 b) ψ ->
+Lemma bindings_pair `{Encode A, Encode B} η p1 p2 e bs (φ : env → Prop) φ'
+  (φ_pair : τ[A;B] -> Prop) ψ :
+  pure (eval η e) φ_pair ψ ->
   bindings η bs φ' ψ ->
-  (∀ a b η', φ1 a -> φ2 b -> φ' η' -> pattern η η' (PPair p1 p2) #(a, b) φ False) ->
+  (∀ ab η', φ_pair ab -> φ' η' -> pattern η η' (PPair p1 p2) #ab φ False) ->
   bindings η (Binding (PPair p1 p2) e :: bs) φ ψ.
 Proof.
   intros Hpure Hbs Hpat.
   eapply bindings_cons; eauto.
-  intros [a b] η' [Hψ1 Hψ2] Hη'.
-  auto.
 Qed.
-
 
 (* -------------------------------------------------------------------------- *)
 
@@ -141,7 +140,7 @@ Proof.
   - exists (δ' ++ δ). simpl in Heq. rewrite <- Heq in Hφ. eauto.
 Qed.
 
-Definition binding `{Encode A} η p e φ ψ :=
+Definition binding `{Encode A} η p e φ (ψ : exn → Prop) :=
   pure (eval η e) (λ a : A, pattern η [] p #a φ False) ψ.
 
 Lemma binding_bindings_conseq `{Encode A} η p e bs (φ1 φ2 φ : env → Prop) ψ :
@@ -176,4 +175,6 @@ Proof.
   apply pure_irrefutably_extend.
   eapply (pattern_app η η' p ♯a φ ⊥).
   apply Hpat_η'.
+  Unshelve. all: eauto with pure.
+  exact _.
 Qed.
